proof/crefine/RISCV64/ADT_C.thy
@@ -1215,7 +1215,7 @@ lemma ksPSpace_eq_imp_valid_pspace'_eq:
   assumes ksPSpace: "ksPSpace s' = ksPSpace s"
   shows "valid_pspace' s = valid_pspace' s'"
   using assms
-  by (clarsimp simp: valid_pspace'_def pspace_aligned'_def
+  by (clarsimp simp: valid_pspace'_def pspace_aligned'_def pspace_in_kernel_mappings'_def
         pspace_distinct'_def ps_clear_def no_0_obj'_def valid_mdb'_def
         pspace_canonical'_def pspace_in_kernel_mappings'_def
         ksPSpace_eq_imp_valid_objs'_eq[OF ksPSpace])
